feat: commit CachedRecognizer to no pointers

Earley/CachedRecognizer.lean
@@ -12,31 +12,17 @@ public import Earley.Recognizer
 public import Mathlib.Data.Set.Card
 
 /-!
-This module represents a computable implementation of the Earley algorithm.
+This module represents a optimized implementation of the Earley algorithm.
+For more details on the general algorithm, see `Recognizer`.
 
-Given an input word `w = a_0 .. a_(n-1)` of length `n`, we maintain a list of `n+1` bins `B_k`.
-For the initial starting position and position after parsing a certain characters,
-we maintain a bin of the possible states we could be in.
-Each bin contains a set of `BinItem`s, which are a pair of an `EarleyItem` and a `Pointer`,
-which help us keep track of its origin. The pointer is only required to assemble the parse tree.
+In comparison to the naive implementation in `Recognizer`:
+- caches if an item already exists in a bin
+- caches the indices for the items that can be completed: HashMap N (i, EarleyItem T N)
+- doesn't maintain pointers to reconstruct a parse tree afterwards
 
-The `endIdx` of an `EarleyItem` corresponds always to the bin number.
-`B_0` is filled with the items from the INIT rule.
-
-The parse tree will only be built _after_ a word has been fully recognized,
-thus the Recognizer has to keep track of all its bins until its done.
-
-The algorithm goes through the bins in ascending order.
-Due to a complication with epsilon rules, `.complete` may miss transitions,
-so Rau only reasons about epsilon free grammars.
-
-This is the cached variant. It adds:
-- an index for the items in a bin, so checking for containment becomes O(1) HashSet (EarleyItem T N)
-- maybe an index for the items that could be completed? HashMap N (i, BinItem T N)
-
-These optimizations do make it such that maintaining only origin information per binitem is way
-more convenient, and since the implementation for `build_tree` only uses the first pointer
-of the reduction pointer anyway, this isn't a big deal.
+These optimizations do make it such that maintaining only origin information per binitem would be
+way more convenient, and since the implementation for `build_tree` only uses the first pointer
+of the reduction pointer anyway, this isn't a big deal. So extending to that makes somewhat sense?
 
 TODO: CachedParser would use `Array.findIdx?` instead of filterWithIdx?
 -/
@@ -66,7 +52,7 @@ abbrev CompletionCache (T N : Type) [BEq N] [Hashable N] : Type :=
 
 public structure CachedEarleyBin (T N : Type) [BEq T] [BEq N] [BEq (EarleyItem T N)]
     [Hashable N] [Hashable (EarleyItem T N)] where
-  raw : Array (Recognizer.BinItem T N)
+  raw : Array (EarleyItem T N)
   items : ItemCache T N
   completions : CompletionCache T N
 
@@ -77,40 +63,50 @@ abbrev CachedEarleyBins (T N : Type) [BEq T] [BEq N] [BEq (EarleyItem T N)]
 variable {T N : Type} [BEq T] [BEq N] [LawfulBEq (EarleyItem T N)] [Hashable N]
   [Hashable (EarleyItem T N)]
 
-@[grind]
-def items (bin : Array (Recognizer.BinItem T N)) : Array (EarleyItem T N) :=
-  bin.map (fun x => x.item)
+--@[grind]
+--def items (bin : Array (Recognizer.BinItem T N)) : Array (EarleyItem T N) :=
+--  bin.map (fun x => x.item)
 
 section WellFormedBin
 
 -- FIXME: I dont merge, so maybe I need less of the invariant?
-@[grind]
-public def isWellFormedPointer (w : List T) (bins : CachedEarleyBins T N (w.length + 1))
-    (pointer : Recognizer.Pointer) (k : Nat) : Prop :=
-  match pointer with
-  | .null => True
-  | .predecessor i => k ≠ 0 ∧ k - 1 ≤ w.length ∧ ((h : k - 1 ≤ w.length) → i < bins[k-1].raw.size)
-  | .reduction p ps => k ≤ w.length ∧ p.endIdxA ≤ w.length ∧
-      ((h : p.endIdxA ≤ w.length) → p.i < bins[p.endIdxA].raw.size) ∧
-      ((h : k ≤ w.length) → p.j < bins[k].raw.size)
+--@[grind]
+--public def isWellFormedPointer (w : List T) (bins : CachedEarleyBins T N (w.length + 1))
+--    (pointer : Recognizer.Pointer) (k : Nat) : Prop :=
+--  match pointer with
+--  | .null => True
+--  | .predecessor i => k ≠ 0 ∧ k - 1 ≤ w.length ∧ ((h : k - 1 ≤ w.length) → i < bins[k-1].raw.size)
+--  | .reduction p ps => k ≤ w.length ∧ p.endIdxA ≤ w.length ∧
+--      ((h : p.endIdxA ≤ w.length) → p.i < bins[p.endIdxA].raw.size) ∧
+--      ((h : k ≤ w.length) → p.j < bins[k].raw.size)
+--
+--@[grind]
+--public def isWellFormedBinPointers (w : List T) (bins : CachedEarleyBins T N (w.length + 1))
+--    (bin : Array (Recognizer.BinItem T N)) (k : Nat) : Prop :=
+--  ∀ x ∈ bin, isWellFormedPointer w bins x.pointer k
 
+/--
+The items of an EarleyBin are well-formed, if
+- there are no duplicate items in the bin
+- all items in the bin are well-formed
+- the endIdx of all items match the index of the bin
+-/
 @[grind]
-public def isWellFormedBinPointers (w : List T) (bins : CachedEarleyBins T N (w.length + 1))
-    (bin : Array (Recognizer.BinItem T N)) (k : Nat) : Prop :=
-  ∀ x ∈ bin, isWellFormedPointer w bins x.pointer k
+public def isWellFormedBinItems (G : ContextFreeGrammarList T N) (w : List T) (k : Nat)
+    (bin : Array (EarleyItem T N)) : Prop :=
+  bin.toList.Nodup ∧ ∀ x ∈ bin, isWellFormed G.rules (mapT w) x ∧ x.endIdx = k
 
 /--
 CachedEarleyBins are well-formed, if all of its bins and its caches are well-formed.
+FIXME: missing pointer invariants
 -/
 @[grind]
 public def isWellFormedCachedBins (G : ContextFreeGrammarList T N) (w : List T)
     (bins : CachedEarleyBins T N (w.length + 1)) : Prop :=
   -- FIXME: missing invariant about the cache stating that the items correspond
   --        to the items in each bin ? Or do I want to prove this separately?
-  ∀ k, (hk : k < bins.size) → Recognizer.isWellFormedBinItems G w k bins[k].raw.toList
-    ∧ isWellFormedBinPointers w bins bins[k].raw k
-    ∧ ∀ j, (hj : j < bins[k].raw.size) → Recognizer.isSoundPointer bins[k].raw[j].pointer k j
-    ∧ sorry
+  ∀ k, (hk : k < bins.size) → isWellFormedBinItems G w k bins[k].raw
+    --∧ sorry
 
 /--
 A combination of an EarleyBins with its cache and a well-formedness Invariant about it.
@@ -120,41 +116,70 @@ public structure WfEarleyBinsCached (G : ContextFreeGrammarList T N) (w : List T
   inv : isWellFormedCachedBins G w bins
 
 /--
+List-based implementation of the .init operation.
+Returns a list filled with all possible .init states.
+-/
+public def initCached (G : ContextFreeGrammarList T N) : List (EarleyItem T N) :=
+  let rules := G.rules.filter (fun r => r.input == G.initial)
+  rules.map (fun r => ⟨r,0,0,0⟩)
+
+/--
+List-based implementation of the .scan operation.
+
+Gets called with the next symbol being the terminal `a` of the item `x` and returns a new item
+if `a` matches the word for given index `k`.
+-/
+public def scanCached (w : List T) (x : EarleyItem T N) (a : T) (k : Nat) (h : k < w.length) :
+    List (EarleyItem T N) :=
+  if w[k] == a then
+    [incItem x (x.endIdx+1)]
+  else
+    []
+
+/--
+List-based implementation of the .predict operation.
+
+Returns a fresh item for each rule, which got `A` as its lhs.
+-/
+public def predictCached (G : ContextFreeGrammarList T N) (A : N) (k : Nat) :
+    List (EarleyItem T N) :=
+  let rules := G.rules.filter (fun r => r.input == A)
+  rules.map (fun r => ⟨r,0,k,k⟩)
+
+/--
 List-based implementation of the .complete operation.
 
 Returns items for each successful completion of item `y` using its startIdx for bins.
-`j` is the index of y in its bin.
 -/
-public def completeCachedList (y : EarleyItem T N) {n : Nat} (bins : CachedEarleyBins T N n)
-    (h : y.startIdx < n) (j : Nat) : List (Recognizer.BinItem T N) :=
+public def completeCached (y : EarleyItem T N) {n : Nat} (bins : CachedEarleyBins T N n)
+    (h : y.startIdx < n) : List (EarleyItem T N) :=
   -- The origin bin filtered for matchings with y
   let xMatches : List (EarleyItem T N × Nat) := bins[y.startIdx].completions.getD y.rule.input []
   -- Matchings mapped onto a new item with the index recorded within the reduction pointer
-  xMatches.map (fun ⟨x,i⟩ => ⟨incItem x y.endIdx, Recognizer.Pointer.reduction ⟨y.startIdx,i,j⟩ []⟩)
+  xMatches.map (fun ⟨x,i⟩ => incItem x y.endIdx)
 
 /--
 Add given list one by one into `xs`, if they are not already part of `xs`.
 -/
 @[inline, grind]
-public def updateBin (xs : CachedEarleyBin T N) :
-    List (Recognizer.BinItem T N) → CachedEarleyBin T N
+public def updateBin (xs : CachedEarleyBin T N) : List (EarleyItem T N) → CachedEarleyBin T N
   | [] => xs
   | y::ys =>
-    if xs.items.contains y.item then
+    if xs.items.contains y then
       updateBin xs ys
     else
       let raw' := xs.raw ++ [y]
-      let items' :=  xs.items.insert y.item
-      match y.item.nextSymbol with
+      let items' :=  xs.items.insert y
+      match y.nextSymbol with
       | some (Symbol.nonterminal n) =>
         match xs.completions[n]? with
         | some _ =>
           -- There exists an entry: append the list with the item of y
           updateBin ⟨raw', items', xs.completions.modify n
-            (fun zs => zs.append [⟨y.item, xs.raw.size⟩])⟩ ys
+            (fun zs => zs.append [⟨y, xs.raw.size⟩])⟩ ys
         | none =>
           -- No entry for `n` yet: create new list for `n` with `y` as first elem.
-          updateBin ⟨raw', items', xs.completions.insert n [⟨y.item, xs.raw.size⟩]⟩ ys
+          updateBin ⟨raw', items', xs.completions.insert n [⟨y, xs.raw.size⟩]⟩ ys
       | _ =>
         -- If the next symbol isn't a non-terminal, the completion cache doesn't need to be touched.
         updateBin ⟨raw', items', xs.completions⟩ ys
@@ -164,9 +189,18 @@ Replace `bins` at index `k` with `newBin` and return the updated bins.
 -/
 @[grind]
 public def updateBinsCached {n : Nat} (bins : CachedEarleyBins T N n) (k : Nat) (hk : k < n)
-    (newBin : List (Recognizer.BinItem T N)) : CachedEarleyBins T N n :=
+    (newBin : List (EarleyItem T N)) : CachedEarleyBins T N n :=
   let updBin := updateBin bins[k] newBin
   bins.set k updBin hk
+
+
+omit [LawfulBEq (EarleyItem T N)] in
+public theorem startIdx_of_Wf {G : ContextFreeGrammarList T N} {w : List T} (x : EarleyItem T N)
+    {bins : CachedEarleyBins T N (w.length + 1)} (hbins : isWellFormedCachedBins G w bins)
+    (k : Nat) (hk : k < w.length + 1) (j : Nat) (hj : j < bins[k].raw.size)
+    (hmemx : x = bins[k].raw[j]) : x.startIdx < w.length + 1 := by
+  have : x ∈ bins[k].raw := by grind
+  grind
 
 end WellFormedBin
 
@@ -181,11 +215,11 @@ public def earleyBinList {G : ContextFreeGrammarList T N} {w : List T}
     ⟨bins, hbins⟩
   else
     let x := bins[k].raw[j]
-    let bins' := match nextSymbol x.item with
+    let bins' := match nextSymbol x with
     | some s => match s with
       | Symbol.nonterminal A =>
         -- Add all potential .predict operations on the current item to the current bin
-        let newItems := Recognizer.predictList G A k
+        let newItems := predictCached G A k
         updateBinsCached bins k hk newItems
       | Symbol.terminal a =>
         -- If we are the final bin then don't try to progress via consuming another terminal
@@ -193,17 +227,26 @@ public def earleyBinList {G : ContextFreeGrammarList T N} {w : List T}
           bins
         else
           -- Add a potential .scan operations on the current item to the next bin
-          let newItem := Recognizer.scanList w x.item a k (by omega) j
+          let newItem := scanCached w x a k (by omega)
           updateBinsCached bins (k+1) (by lia) newItem
     | none =>
       -- Add all potential .complete operations on the current item to the current bin
-      let newItems := completeCachedList x.item bins (by sorry) j
+      let newItems := completeCached x bins (by grind [startIdx_of_Wf x hbins])
       updateBinsCached bins k hk newItems
     have : isWellFormedCachedBins G w bins' := by sorry
     earleyBinList bins' k (by omega) (j+1) this
 termination_by { x | isWellFormed G.rules (mapT w) x }.ncard + 1 - j
-decreasing_by --exact decreasingAux hbins j k (by lia) (by lia)
-  sorry
+decreasing_by
+  apply Nat.sub_lt_sub_left
+  · specialize hbins k (by lia)
+    let wfItemsBin := { x | isWellFormed G.rules (mapT w) x }
+    have : bins[k].raw.size ≤ wfItemsBin.ncard := by
+      have hF := Earley.Proofs.Finiteness.finiteEarleyWF G (mapT w)
+      let P := (fun x => isWellFormed G.rules (mapT w) x)
+      apply Recognizer.length_lte_ncard_of_superset bins[k].raw.toList wfItemsBin P
+        (by grind) (by grind) hbins.left
+    grind
+  · simp
 
 /--
 Initialize bins by constructing the first bin through using .init for all G.rules.
@@ -214,7 +257,7 @@ TODO: I could use of Std.HashSet.ofList and something more clever for the HashMa
 public def initCachedBins (G : ContextFreeGrammarList T N) (w : List T) : WfEarleyBinsCached G w :=
   let bins : Vector (CachedEarleyBin T N) (w.length + 1) :=
     Vector.replicate (w.length + 1) ⟨Array.empty,  {},  {}⟩
-  let bins' := updateBinsCached bins 0 (by lia) (Recognizer.initList G)
+  let bins' := updateBinsCached bins 0 (by lia) (initCached G)
   ⟨bins', (by sorry)⟩ --grind [initList, wfBinItems_of_initList])⟩
 
 /--
@@ -248,7 +291,7 @@ TODO: what code gets compiled from `∃ x ∈ List ?
 @[grind]
 public def recognizeList (G : ContextFreeGrammarList T N) (w : List T) [LawfulBEq T] : Bool :=
   let bins := earleyList G w |>.bins
-  let finalItems := bins[w.length].raw.map (fun x => x.item)
+  let finalItems := bins[w.length].raw
   ∃ x ∈ finalItems, isFinished G.initial (mapT w) x
 
 end CachedRecognizer
